crates/utils/intrinsics/src/avx2.rs
@@ -52,15 +52,19 @@ pub fn mm256_storeu_si256_i16(output: &mut [i16], vector: Vec256) {
     extra::mm256_storeu_si256_i16_model(output, vector)
 }
 
-#[hax_lib::opaque]
 #[hax_lib::ensures(|_r| future(output).len() == output.len())]
+#[cfg_attr(hax, hax_lib::fstar::before(r#"[@@ "opaque_to_smt"]"#))]
 #[inline(always)]
 pub fn mm256_storeu_si256_i32(output: &mut [i32], vector: Vec256) {
     #[cfg(not(hax))]
-    debug_assert_eq!(output.len(), 8);
-    unsafe {
-        _mm256_storeu_si256(output.as_mut_ptr() as *mut Vec256, vector);
+    {
+        debug_assert_eq!(output.len(), 8);
+        unsafe {
+            _mm256_storeu_si256(output.as_mut_ptr() as *mut Vec256, vector);
+        }
     }
+    #[cfg(hax)]
+    extra::mm256_storeu_si256_i32_model(output, vector)
 }
 
 #[hax_lib::ensures(|_r| future(output).len() == output.len())]
@@ -97,15 +101,19 @@ pub fn mm_storeu_si128_u8(output: &mut [u8], vector: Vec128) {
     }
 }
 
-#[hax_lib::opaque]
 #[hax_lib::ensures(|_r| future(output).len() == output.len())]
+#[cfg_attr(hax, hax_lib::fstar::before(r#"[@@ "opaque_to_smt"]"#))]
 #[inline(always)]
 pub fn mm_storeu_si128_i32(output: &mut [i32], vector: Vec128) {
     #[cfg(not(hax))]
-    debug_assert_eq!(output.len(), 4);
-    unsafe {
-        _mm_storeu_si128(output.as_mut_ptr() as *mut Vec128, vector);
+    {
+        debug_assert_eq!(output.len(), 4);
+        unsafe {
+            _mm_storeu_si128(output.as_mut_ptr() as *mut Vec128, vector);
+        }
     }
+    #[cfg(hax)]
+    extra::mm_storeu_si128_i32_model(output, vector)
 }
 
 #[hax_lib::ensures(|_r| future(output).len() == output.len())]
@@ -165,12 +173,16 @@ pub fn mm256_loadu_si256_i16(input: &[i16]) -> Vec256 {
     extra::mm256_loadu_si256_i16_model(input)
 }
 
-#[hax_lib::opaque]
+#[cfg_attr(hax, hax_lib::fstar::before(r#"[@@ "opaque_to_smt"]"#))]
 #[inline(always)]
 pub fn mm256_loadu_si256_i32(input: &[i32]) -> Vec256 {
     #[cfg(not(hax))]
-    debug_assert_eq!(input.len(), 8);
-    unsafe { _mm256_loadu_si256(input.as_ptr() as *const Vec256) }
+    {
+        debug_assert_eq!(input.len(), 8);
+        unsafe { _mm256_loadu_si256(input.as_ptr() as *const Vec256) }
+    }
+    #[cfg(hax)]
+    extra::mm256_loadu_si256_i32_model(input)
 }
 
 #[inline(always)]
